Proved computation graphs always compute a value, and are deterministic.
This is subject to the requirement that the graphs be well-formed.

Next step is to show that any for loop will give rise to a well-formed
computation graph that computes the same value. After that, I will
need to show that if we have a good \delta to hand, then the graph
will be the same.

hol/datadepsScript.sml
@@ -3,6 +3,7 @@ open primitivesTheory forLoopTheory pred_setTheory
 open lcsymtacs
 
 fun asimp thl = asm_simp_tac (srw_ss() ++ ARITH_ss) thl
+fun dsimp thl = asm_simp_tac (srw_ss() ++ boolSimps.DNF_ss) thl
 
 val _ = new_theory "datadeps";
 
@@ -11,38 +12,219 @@ val eval_def = Define`
     update A (Wf i) (vf i (MAP (λf. vsub A (f i)) Rs))
 `;
 
-val _ = type_abbrev("action", ``:num # num list # ('a list -> 'a)``)
+val _ = Hol_datatype`
+  action = <|
+    write : num ;
+    reads : num list ;
+    expr : 'a list -> 'a;
+    iter : num
+  |>
+`;
 
 val apply_action_def = Define`
-  apply_action ((w,rs,f) : 'a action) (A:'a mvector) =
-    update A w (f (MAP (vsub A) rs))
+  apply_action (a:'a action) (A:'a mvector) =
+    update A a.write (a.expr (MAP (vsub A) a.reads))
 `;
 
 val touches_def = Define`
-  touches (w1,rs1,f1) (w2,rs2,f2) ⇔
-     w1 = w2 ∨ MEM w1 rs2 ∨ MEM w2 rs1
+  touches a1 a2 ⇔
+     a1.write = a2.write ∨ MEM a1.write a2.reads ∨ MEM a2.write a1.reads
 `;
+
+val MAP_vsub = store_thm(
+  "MAP_vsub",
+  ``¬MEM w reads ⇒ MAP ($' (update A w e)) reads = MAP ($' A) reads``,
+  Induct_on `reads` >> simp[update_sub]);
+
+val nontouching_actions_commute = store_thm(
+  "nontouching_actions_commute",
+  ``¬touches a1 a2 ⇒
+    apply_action a1 (apply_action a2 A) = apply_action a2 (apply_action a1 A)``,
+  simp[touches_def, apply_action_def, vector_EQ] >> rpt strip_tac >>
+  map_every qabbrev_tac [`w1 = a1.write`, `w2 = a2.write`] >>
+  ONCE_REWRITE_TAC [update_sub] >> simp[] >>
+  Cases_on `i = w1` >> simp[]
+  >- (simp[SimpRHS, update_sub] >>
+      reverse (Cases_on `w1 < vsz A`) >>
+      simp[update_sub, MAP_vsub]) >>
+  simp[update_sub, MAP_vsub]);
+
+
+
+val touches_REFL = store_thm(
+  "touches_REFL",
+  ``touches a a``,
+  simp[touches_def]);
+val _ = export_rewrites ["touches_REFL"]
 
 val touches_SYM = store_thm(
   "touches_SYM",
   ``touches a1 a2 ⇒ touches a2 a1``,
-  map_every qid_spec_tac [`a1`, `a2`] >>
-  simp[pairTheory.FORALL_PROD, touches_def] >>
-  rpt strip_tac >> simp[]);
+  simp[touches_def] >> rpt strip_tac >> simp[]);
 
 val wfG_def = Define`
   wfG (els,R) ⇔
+      FINITE els ∧
       (∀a1 a2. R a1 a2 ⇒ touches a1 a2 ∧ a1 ∈ els ∧ a2 ∈ els) ∧
-      ∀a1 a2. a1 ∈ els ∧ a2 ∈ els ∧ touches a1 a2 ⇒ (¬R a1 a2 ⇔ R a2 a1) ∧
+      (∀a1 a2. a1 ∈ els ∧ a2 ∈ els ∧ touches a1 a2 ∧ a1 ≠ a2 ⇒ (¬R a1 a2 ⇔ R a2 a1)) ∧
       ∀a1 a2. a1 ∈ els ∧ a2 ∈ els ∧ R⁺ a1 a2 ⇒ ¬R⁺ a2 a1
 `;
+
+val wfG_irrefl = store_thm(
+  "wfG_irrefl",
+  ``wfG (es,R) ∧ x ∈ es ⇒ ¬R x x``,
+  simp[wfG_def] >> rpt strip_tac >>
+  metis_tac[relationTheory.TC_SUBSET]);
+
+val wfGs_pull_apart = store_thm(
+  "wfGs_pull_apart",
+  ``wfG (a INSERT as, R) ∧ (∀a'. a' ∈ as ⇒ ¬R a' a) ∧ a ∉ as ⇒
+    wfG (as, R \\ a)``,
+  simp[wfG_def] >> rw[] >>
+  metis_tac[relationTheory.TC_MONOTONE, relationTheory.RDOM_DELETE_DEF]);
+
+val _ = IndDefLib.export_rule_induction "relation.TC_STRONG_INDUCT"
+val TC_in_R = store_thm(
+  "TC_in_R",
+  ``∀x y. R⁺ x y ⇒ (∃z. R x z) ∧ (∃z. R z y)``,
+  Induct_on `R⁺ x y` >> metis_tac[]);
+
+val wfG_WF = store_thm(
+  "wfG_WF",
+  ``wfG (es, R) ⇒ WF R``,
+  simp[wfG_def] >> strip_tac >>
+  `R = REL_RESTRICT R es`
+    by (simp[REL_RESTRICT_DEF, FUN_EQ_THM, EQ_IMP_THM] >>
+        metis_tac[]) >>
+  first_assum (fn th => simp[FINITE_WF_noloops, Once th]) >>
+  pop_assum (SUBST_ALL_TAC o SYM) >>
+  simp[relationTheory.irreflexive_def] >> metis_tac[TC_in_R]);
+
+val wfG_FINITE = store_thm(
+  "wfG_FINITE",
+  ``wfG (es,R) ⇒ FINITE es``,
+  simp[wfG_def]);
+
+val nonempty_wfG_has_points = store_thm(
+  "nonempty_wfG_has_points",
+  ``wfG (es, R) ∧ es ≠ ∅ ⇒
+    ∃e. e ∈ es ∧ ∀e'. e' ∈ es ⇒ ¬R e' e``,
+  rpt strip_tac >>
+  `WF R` suffices_by
+    (simp[relationTheory.WF_DEF, IN_DEF] >>
+     pop_assum mp_tac >> simp[GSYM MEMBER_NOT_EMPTY, IN_DEF] >>
+     metis_tac[]) >>
+  metis_tac[wfG_WF]);
 
 val (evalG_rules,evalG_ind,evalG_cases) = Hol_reln`
   (∀A R. evalG A (∅, R) A) ∧
   (∀a as A0 A R.
-      (∀a'. a' ∈ as ⇒ ¬touches a a') ∧ a ∉ as ∧
-      evalG (apply_action a A0) (as, R) A ⇒
-      evalG A0 (a INSERT as, R)
+      (∀a'. a' ∈ as ⇒ ¬R a' a) ∧ a ∉ as ∧
+      evalG (apply_action a A0) (as, R \\ a) A ⇒
+      evalG A0 (a INSERT as, R) A)
+`;
+
+val evalG_EMPTY = store_thm(
+  "evalG_EMPTY",
+  ``evalG A0 (∅, R) A ⇔ A = A0``,
+  simp[Once evalG_cases]);
+val _ = export_rewrites ["evalG_EMPTY"]
+
+val INSERT_11 = store_thm(
+  "INSERT_11",
+  ``e ∉ s1 ∧ e ∉ s2 ⇒ (e INSERT s1 = e INSERT s2 ⇔ s1 = s2)``,
+  simp[EQ_IMP_THM] >> simp[EXTENSION] >> metis_tac[]);
+
+val evalG_total = store_thm(
+  "evalG_total",
+  ``wfG G ⇒ ∃A'. evalG A G A'``,
+  pairLib.PairCases_on `G` >> map_every qabbrev_tac [`es = G0`, `R = G1`] >>
+  markerLib.RM_ALL_ABBREVS_TAC >>
+  map_every qid_spec_tac [`A`, `R`] >>
+  Induct_on `CARD es`
+  >- (simp[Once evalG_cases] >> metis_tac[CARD_EQ_0, wfG_def]) >>
+  qx_gen_tac `es` >> strip_tac >>
+  `es ≠ ∅` by (strip_tac >> fs[]) >>
+  map_every qx_gen_tac [`R`, `A0`] >> strip_tac >>
+  `∃e. e ∈ es ∧ ∀e'. e' ∈ es ⇒ ¬R e' e` by metis_tac[nonempty_wfG_has_points] >>
+  `∃es0. e ∉ es0 ∧ es = e INSERT es0` by metis_tac[DECOMPOSITION] >>
+  `FINITE es` by fs[wfG_def] >> rw[] >> fs[] >>
+  first_x_assum (qspec_then `es0` mp_tac) >> simp[] >>
+  disch_then (qspecl_then [`R \\ e`, `apply_action e A0`] mp_tac) >>
+  `wfG (es0, R \\ e)` by metis_tac[wfGs_pull_apart] >> simp[] >>
+  disch_then (qx_choose_then `A0'` assume_tac) >>
+  metis_tac[evalG_rules]);
+
+val wfG_evaluate_deterministically = store_thm(
+  "wfG_evaluate_deterministically",
+  ``wfG G ∧ evalG A0 G A ⇒
+    ∀A'. evalG A0 G A' ⇒ A' = A``,
+  pairLib.PairCases_on `G` >> map_every qabbrev_tac [`es = G0`, `R = G1`] >>
+  markerLib.RM_ALL_ABBREVS_TAC >>
+  map_every qid_spec_tac [`A0`, `A`, `R`] >>
+  completeInduct_on `CARD es` >>
+  qx_gen_tac `es` >>
+  qmatch_rename_tac `n = CARD es ⇒ XX` ["XX"] >> strip_tac >>
+  map_every qx_gen_tac [`R`, `A`, `A0`] >> strip_tac >>
+  qx_gen_tac `A'` >> strip_tac >>
+  full_simp_tac (srw_ss() ++ boolSimps.DNF_ss)
+    [AND_IMP_INTRO, GSYM CONJ_ASSOC] >> rw[] >>
+  qpat_assum `evalG A0 (es, R) A` mp_tac >>
+  simp[Once evalG_cases] >>
+  disch_then (DISJ_CASES_THEN2
+                strip_assume_tac
+                (qx_choosel_then [`e1`, `es1`] strip_assume_tac))
+  >- fs[] >>
+  qpat_assum `evalG XX YY A'` mp_tac >>
+  simp[Once evalG_cases] >>
+  disch_then (qx_choosel_then [`e2`, `es2`] strip_assume_tac) >>
+  Cases_on `e2 = e1`
+  >- (rw[] >>
+      `es2 = es1` by metis_tac[INSERT_11] >>
+      rw[] >>
+      `FINITE es1` suffices_by
+        (strip_tac >> fs[] >>
+         metis_tac[DECIDE ``x < SUC x``, wfGs_pull_apart]) >>
+      fs[wfG_def]) >>
+  `e1 ∈ es2 ∧ e2 ∈ es1` by metis_tac[EXTENSION, IN_INSERT] >>
+  `∃es0. es1 = e2 INSERT es0 ∧ es2 = e1 INSERT es0 ∧ e1 ∉ es0 ∧ e2 ∉ es0`
+    by (`∃es0. es1 = e2 INSERT es0 ∧ e2 ∉ es0` by metis_tac[DECOMPOSITION] >>
+        qexists_tac `es0` >> simp[] >> fs[] >>
+        qpat_assum `XX INSERT YY INSERT ZZ = UU INSERT VV` mp_tac >>
+        ONCE_REWRITE_TAC [INSERT_COMM] >> simp[INSERT_11]) >>
+  rw[] >>
+  `wfG (e2 INSERT es0, R \\ e1) ∧ wfG (es0, R \\ e2 \\ e1) ∧
+   wfG (e1 INSERT es0, R \\ e2) ∧ wfG (es0, R \\ e1 \\ e2)`
+    by metis_tac[wfGs_pull_apart, IN_INSERT, relationTheory.RDOM_DELETE_DEF] >>
+  `FINITE es0` by metis_tac[wfG_FINITE] >>
+  `(∃A21. evalG (apply_action e1 (apply_action e2 A0)) (es0, R \\ e2 \\ e1) A21) ∧
+   ∃A12. evalG (apply_action e2 (apply_action e1 A0)) (es0, R \\ e1 \\ e2) A12`
+    by metis_tac[evalG_total] >>
+  `evalG (apply_action e2 A0) (e1 INSERT es0, R \\ e2) A21 ∧
+   evalG (apply_action e1 A0) (e2 INSERT es0, R \\ e1) A12`
+    by metis_tac[evalG_rules, IN_INSERT, relationTheory.RDOM_DELETE_DEF] >>
+  `A' = A21 ∧ A = A12`
+    by (conj_tac >>
+        first_x_assum match_mp_tac >| [
+          qexists_tac `e1 INSERT es0`,
+          qexists_tac `e2 INSERT es0`
+        ]>> simp[] >> metis_tac[]) >>
+  ntac 2 (pop_assum SUBST_ALL_TAC) >>
+  `R \\ e2 \\ e1 = R \\ e1 \\ e2`
+    by (simp[FUN_EQ_THM, relationTheory.RDOM_DELETE_DEF] >> metis_tac[]) >>
+  pop_assum SUBST_ALL_TAC >>
+  `apply_action e1 (apply_action e2 A0) = apply_action e2 (apply_action e1 A0)`
+    suffices_by (disch_then SUBST_ALL_TAC >> first_x_assum match_mp_tac >>
+                 qexists_tac `es0` >> simp[] >> metis_tac[]) >>
+  `¬R e2 e1 ∧ ¬R e1 e2` by metis_tac[] >>
+  `¬touches e1 e2`
+    by (qpat_assum `wfG (e1 INSERT e2 INSERT es0, R)` mp_tac >>
+        simp[wfG_def] >> metis_tac[]) >>
+  match_mp_tac nontouching_actions_commute >> simp[]);
+
+
+
+
 
 
 
